SimpleAuction.fst
@@ -1,0 +1,175 @@
+
+(******************)
+module SimpleAuction
+open FStar.All
+open FStar.UInt160
+open FStar.UInt256
+open FStar.Heap
+open FStar.List
+open FStar.UInt
+
+type msg = {
+  sender : UInt160.t;
+  value: UInt256.t;
+  now : UInt256.t;
+}
+
+val set : #key:eqtype -> #vl:Type -> (key -> vl) -> key -> vl -> (key -> vl)
+let set #key #vl f ind x ind2 = if ind = ind2 then x else f ind2
+
+val get : #key:eqtype -> #vl:Type -> (key -> vl) -> key -> vl
+let get #key #vl f ind = f ind
+
+val address_to_uint : UInt160.t -> UInt256.t
+let address_to_uint a =
+  let x : uint_t 160 = UInt160.v a in
+  let y : uint_t 256 = UInt.to_uint_t 256 x in
+  UInt256.uint_to_t y
+
+val uint_to_address : UInt256.t -> UInt160.t
+let uint_to_address a = UInt160.uint_to_t (UInt.to_uint_t 160 (UInt256.v a))
+
+val list_length : #a:Type -> list a -> UInt256.t
+let list_length #a lst = UInt256.uint_to_t (UInt.to_uint_t 256 (List.length lst))
+
+val list_nth : #a:Type -> list a -> UInt256.t -> ML a
+let list_nth #a lst n = List.nth lst (UInt256.v n)
+
+val list_set : #a:Type -> list a -> UInt256.t -> a -> ML (list a)
+let list_set #a lst n elem =
+  let n = UInt256.v n in
+  List.mapi (fun i a -> if i = n then elem else a) lst 
+
+exception SolidityThrow
+exception SolidityReturn
+exception SolidityBadReturn
+
+val do_call : #state:Type -> #ret:Type -> (state -> ML (option ret * state)) -> state -> ML (option ret * state)
+let do_call #state #ret meth st =
+  try meth st
+  with SolidityThrow -> (None, st)
+
+val bool_and : bool -> bool -> Tot bool
+let bool_and a b = a && b
+
+val bool_or : bool -> bool -> Tot bool
+let bool_or a b = a || b
+
+type event =
+|HighestBidIncreased : UInt160.t -> UInt256.t -> event
+|AuctionEnded : UInt160.t -> UInt256.t -> event
+
+
+(* Storage state *)
+noeq type state = {
+events: list event;
+beneficiary : UInt160.t;
+auctionStart : UInt256.t;
+biddingTime : UInt256.t;
+highestBidder : UInt160.t;
+highestBid : UInt256.t;
+pendingReturns : UInt160.t -> UInt256.t;
+ended : bool;
+}
+val method_HighestBidIncreased : msg -> state -> UInt160.t -> UInt256.t -> ML (option unit * state)
+let method_HighestBidIncreased msg state bidder amount =
+ let state = {state with events = HighestBidIncreased bidder amount :: state.events} in
+(Some (), state)
+
+val method_AuctionEnded : msg -> state -> UInt160.t -> UInt256.t -> ML (option unit * state)
+let method_AuctionEnded msg state winner amount =
+ let state = {state with events = AuctionEnded winner amount :: state.events} in
+(Some (), state)
+
+let address_0 = UInt160.uint_to_t (0)
+let uint256_0 = UInt256.uint_to_t (0)
+
+
+
+
+
+
+
+(* Contract methods *)
+val method_SimpleAuction : msg -> state -> UInt256.t -> UInt160.t -> ML (option (unit) * state)
+let method_SimpleAuction msg state _biddingTime _beneficiary =
+let s = alloc state in
+let ret = alloc None in
+try
+s := {!s with beneficiary = (_beneficiary) };
+s := {!s with auctionStart = (msg.now) };
+s := {!s with biddingTime = (_biddingTime) };
+(!ret, !s)
+with SolidityReturn -> (!ret, !s)
+
+
+val method_bid : msg -> state -> unit -> ML (option (unit) * state)
+let method_bid msg state () =
+let s = alloc state in
+let ret = alloc None in
+try
+if UInt256.gt (msg.now) (UInt256.add_mod ((!s).auctionStart) ((!s).biddingTime))
+then (raise SolidityThrow; ())
+else ();
+
+if UInt256.lte ((msg).value) ((!s).highestBid)
+then (raise SolidityThrow; ())
+else ();
+
+if op_disEquality ((!s).highestBidder) (address_0)
+then (s := {!s with pendingReturns = set (!s).pendingReturns ((!s).highestBidder) (UInt256.add_mod ((get (!s).pendingReturns ((!s).highestBidder))) ((!s).highestBid)) }; ())
+else ();
+
+s := {!s with highestBidder = ((msg).sender) };
+s := {!s with highestBid = ((msg).value) };
+(let (ret__,st__) = method_HighestBidIncreased msg !s
+(msg).sender(msg).value in
+ (s := st__; match ret__ with Some x -> x | None -> (* assert False ; *) raise SolidityBadReturn));
+(!ret, !s)
+with SolidityReturn -> (!ret, !s)
+
+
+val method_withdraw : msg -> state -> unit -> ML (option (bool) * state)
+let method_withdraw msg state () =
+let s = alloc state in
+let ret = alloc None in
+try
+let amount = alloc ((get (!s).pendingReturns ((msg).sender))) in
+
+if UInt256.gt (!amount) (uint256_0)
+then (s := {!s with pendingReturns = set (!s).pendingReturns ((msg).sender) (uint256_0) };
+if op_Negation (false)
+then (s := {!s with pendingReturns = set (!s).pendingReturns ((msg).sender) (!amount) };
+ret := Some(false); raise SolidityReturn; ())
+else ();
+ ())
+else ();
+
+ret := Some(true); raise SolidityReturn;
+(!ret, !s)
+with SolidityReturn -> (!ret, !s)
+
+
+val method_auctionEnd : msg -> state -> unit -> ML (option (unit) * state)
+let method_auctionEnd msg state () =
+let s = alloc state in
+let ret = alloc None in
+try
+if UInt256.lte (msg.now) (UInt256.add_mod ((!s).auctionStart) ((!s).biddingTime))
+then (raise SolidityThrow; ())
+else ();
+
+if (!s).ended
+then (raise SolidityThrow; ())
+else ();
+
+s := {!s with ended = (true) };
+(let (ret__,st__) = method_AuctionEnded msg !s
+(!s).highestBidder(!s).highestBid in
+ (s := st__; match ret__ with Some x -> x | None -> (* assert False ; *) raise SolidityBadReturn));
+if op_Negation (false)
+then (raise SolidityThrow; ())
+else ();
+
+(!ret, !s)
+with SolidityReturn -> (!ret, !s)
